im kmsing why am i still in week 2

week2/problems/problem3.dfy
@@ -10,11 +10,12 @@ method GCD(a: int, b: int) returns (gcd: int)
     var x := a;
     var y := b;
     
+    
     while y > 0 // changed, since "decreases expression must be bounded below by 0 at end of loop iteration"
 
         invariant x >= 1
         invariant y >= 0
-        invariant trivial_gcd(a,b,1,1) == trivial_gcd(x,y,1,1)
+        invariant gcd_helper(a,b) == gcd_helper(x,y)
         // (see pg 19, CSUR14.pdf - this problem has been fully outlined)
 
         decreases y
@@ -29,32 +30,15 @@ method GCD(a: int, b: int) returns (gcd: int)
 
 // inspired by the upcoming problems, i will use Helper Function(s)
 
-
-function min(a:int, b:int): int
+function gcd_helper(a:int, b:int): int
+    requires a >= 0 && b >= 0
+    requires a + b > 0
+    ensures gcd_helper(a,b) > 0
+    ensures a % gcd_helper(a,b) == 0 && b % gcd_helper(a,b) == 0
+    ensures forall d :: d > 0 && a % d == 0 && b % d == 0 ==> d <= gcd_helper(a,b)
+    decreases b
 {
-    if a < b then a else b
+    if b == 0 then a
+    else gcd_helper(b, a % b)
 }
-
-
-// the following is a trivial implementation of gcd which is tail recursive
-// (iterative, but dafny can verify via induction without needing invariants)
-
-function trivial_gcd(a: int, b: int, gcd: int, k: int): int
-  requires a >= 0 && b >= 0
-  requires k > 0 && gcd > 0
-  requires k <= min(a, b) + 1
-  ensures trivial_gcd(a, b, gcd, k) > 0
-  decreases min(a, b) - k + 1
-{
-  if k <= min(a, b) then
-    if a % k == 0 && b % k == 0 then
-      trivial_gcd(a, b, k, k+1)
-    else
-      trivial_gcd(a, b, gcd, k+1)
-  else
-    gcd
-}
-
-lemma 
-
 
